AwsCryptographyPrimitives/src/ErrorUtils.dfy
@@ -1,0 +1,29 @@
+// Copyright Amazon.com Inc. or its affiliates. All Rights Reserved.
+// SPDX-License-Identifier: Apache-2.0
+
+include "../Model/AwsCryptographyPrimitivesTypes.dfy"
+
+module {:options "/functionSyntax:4"} ErrorUtils {
+  import opened Wrappers
+  import Types = AwsCryptographyPrimitivesTypes
+
+  function ExtractMessageFromError(
+    error: Types.Error
+  ): (errorMessage?: Option<string>)
+  {
+    match error {
+      case Opaque(obj) => None
+      case AwsCryptographicPrimitivesError(s) => Some(s)
+      case OpaqueWithText(obj, objMessage) => Some(objMessage)
+      case CollectionOfErrors(_, s) => Some(s)
+    }
+  }
+
+  function MessageOrUnknown(
+    error: Types.Error
+  ): (errorMessage: string)
+  {
+    var msg? := ExtractMessageFromError(error);
+    if msg?.Some? then msg?.value else " unkown."
+  }
+}
